user 5, session 19, part 5

diffs-annotated/5/user-5-session-19.v
@@ -34,7 +34,7 @@ Record EpsilonLogic :=
           evalChoose :
            forall env x P,
            (exists value, eval (extendEnv env x value) P = vTrue) ->
-           exists out, eval env (Eq (Choose x P) out) = vTrue;
+           eval (extendEnv env x (eval env (Choose x P))) P = vTrue;
           evalChooseDet :
            forall env x P Q,
            eval env P = vTrue <-> eval env Q = vTrue ->
@@ -57,4 +57,29 @@ Theorem eval_eq_true_or_false :
 Proof.
 (intros).
 (destruct (L.(value_eq_dec) (L.(eval) env t1) (L.(eval) env t2)) eqn:E).
+-
+left.
 (apply L.(evalEqTrue)).
+assumption.
+-
+right.
+(apply L.(evalEqFalse)).
+assumption.
+Qed.
+Theorem identity_correct :
+  forall (L : EpsilonLogic) (t : Term), isTheorem L (Eq t (identity t)).
+Proof.
+(unfold isTheorem).
+(induction t; intros; simpl in *).
+-
+(apply evalEqTrue).
+reflexivity.
+-
+(apply evalEqTrue).
+reflexivity.
+-
+(apply evalEqTrue).
+specialize IHt1 with env.
+specialize IHt2 with env.
+(apply evalEqTrue in IHt1).
+(apply evalEqTrue in IHt2).
